code/hash/Hacl.Impl.SHA2.Core.fsti
@@ -15,6 +15,7 @@ val sha256: hash:lbuffer uint8 32ul -> len:size_t -> b:lbuffer uint8 len ->
     (requires (fun h0 -> live h0 b /\ live h0 hash /\ disjoint hash b))
     (ensures (fun h0 _ h1 -> modifies (loc hash) h0 h1))
 
+
 val sha256_4: r0:lbuffer uint8 32ul ->
               r1:lbuffer uint8 32ul ->
               r2:lbuffer uint8 32ul ->
